fully prove and use release left-moverness
one trick: make [Release] always-enabled by adding nilpotent transitions
when Release is called but the lock is not held by the caller (i.e., Release
does nothing when called in that context).

next step is to prove, in ExampleProtocol.v, that this is a safe plan: i.e.,
if programs follow our locking syntactic rules, they will never call [Release]
in a way that triggers these nilpotent transitions.

src/Spec/Compile.v
@@ -461,6 +461,11 @@ Section Movers.
   Variable moverT : Type.
   Variable opMover : opT moverT.
 
+  Definition always_enabled :=
+    forall tid s,
+      exists r s',
+        op_step opMover tid s r s'.
+
   Definition right_mover :=
     forall `(op1 : opT T2) tid0 tid1 s s0 s1 v0 v1,
       tid0 <> tid1 ->
@@ -471,6 +476,7 @@ Section Movers.
         op_step opMover tid0 s' v0 s1.
 
   Definition left_mover :=
+    always_enabled /\
     forall `(op0 : opT T0) tid0 tid1 s s0 s1 v0 v1,
       tid0 <> tid1 ->
       op_step op0 tid0 s v0 s0 ->
@@ -521,6 +527,7 @@ Section Movers.
     - edestruct IHatomic_exec2; eauto.
       edestruct IHatomic_exec1; intuition eauto.
     - edestruct H.
+      edestruct H4.
       3: eauto.
       2: eauto.
       eauto.
@@ -556,6 +563,7 @@ Section Movers.
     intros.
     induction H1; simpl; eauto.
     - edestruct H.
+      edestruct H4.
       3: eauto.
       2: eauto.
       eauto.
@@ -603,8 +611,12 @@ Section Movers.
           eauto.
           rewrite thread_upd_upd_ne; eauto.
 
-    - admit.
-  Admitted.
+    - destruct H.
+      edestruct H; repeat deex.
+      do 2 eexists; split.
+      eauto.
+      eauto.
+  Qed.
 
   Theorem hitrace_incl_atomize_opexec_right_mover :
     right_mover ->
@@ -755,7 +767,32 @@ Section Movers.
     reflexivity.
 
     rewrite <- hitrace_incl_atomize_opret_ret_l.
-  Admitted.
+
+    repeat rewrite exec_equiv_bind_bind.
+    rewrite <- hitrace_incl_atomize_opexec_ret_left_mover by eauto.
+
+    repeat rewrite exec_equiv_bind_bind.
+    rewrite <- hitrace_incl_atomize_opcall_ret_l.
+
+    repeat rewrite exec_equiv_bind_bind.
+    eapply hitrace_incl_bind_a; intros.
+
+    repeat rewrite exec_equiv_bind_bind with (p1 := OpCall _).
+    eapply hitrace_incl_bind_a; intros.
+
+    rewrite exec_equiv_ret_bind.
+    repeat rewrite exec_equiv_bind_bind with (p1 := OpExec _).
+    eapply hitrace_incl_bind_a; intros.
+
+    rewrite exec_equiv_ret_bind.
+    repeat rewrite exec_equiv_bind_bind with (p1 := OpRet _).
+    eapply hitrace_incl_bind_a; intros.
+
+    rewrite exec_equiv_ret_bind.
+    rewrite exec_equiv_ret_bind.
+    simpl.
+    reflexivity.
+  Qed.
 
 End Movers.
 
